
$1.$ $$\frac{1}{2}+\sum\limits_{k=1}^{n}\cos kx=\frac{\sin(n+\frac{1}{2})x}{2\sin\frac{x}{2}}$$**[证明]**:
	$\begin{align}2\sin\frac{x}{2}(\frac{1}{2}+\sum\limits_{k=1}^{n}\cos kx)&=\sin\frac{x}{2}+\sum\limits_{k=1}^{n}2\sin\frac{x}{2}\cos kx=\sin\frac{x}{2}+\sum\limits_{k=1}^{n}(\sin(\frac{1}{2}+k)x+\sin(\frac{1}{2}-k))\\&=\sin\frac{1}{2}+\sum\limits_{k=1}^{n}(\sin(k+\frac{1}{2})-\sin(k-\frac{1}{2}))=\sin(n+\frac{1}{2})x\end{align}$ 

$2.$ $$\frac{1}{2}+\sum\limits_{k=1}^{n}\sin kx=$$**[证明]**:
	$2\cos\frac{x}{2}(\frac{1}{2}+\sum\limits_{k=1}^{n}\sin kx)=\cos\frac{x}{2}$ 